Temporal_Planning_Base/Base.thy
@@ -104,12 +104,270 @@ fun list_max_opt::"('a::linorder) list \<Rightarrow> 'a option" where
 "list_max_opt [] = None" |
 "list_max_opt (x#xs) = Some (list_max_opt' xs x)"
 
-function upto_aux_nat::"nat \<Rightarrow> nat \<Rightarrow> nat list" where
-"upto_aux_nat m n = (if (m < n) then m#upto_aux_nat (m+1) n else [])"
-  by auto
-termination by (relation "measure (\<lambda>(x, y). y - x)") auto
 
-definition "upto_nat \<equiv> upto_aux_nat 0"
+                                       
+fun fun_upd_lists::"('a \<Rightarrow> 'b) \<Rightarrow> 'a list \<Rightarrow> 'b list \<Rightarrow> ('a \<Rightarrow> 'b)" where
+"fun_upd_lists f [] ys = f" |
+"fun_upd_lists f (x # xs) (y # ys) = fun_upd_lists (f(x := y)) xs ys" |
+"fun_upd_lists f _ _ = f"
+
+
+fun list_of'::"'a \<Rightarrow> nat \<Rightarrow> 'a list \<Rightarrow> 'a list" where
+"list_of' x 0 xs = xs" |
+"list_of' x (Suc n) xs = list_of' x n (x#xs)"
+
+definition "list_of x n = list_of' x n []"
+
+lemma length_list_of': "length (list_of' x n xs) = n + length xs"
+  apply (induction n arbitrary: xs)
+  by auto
+
+lemma length_list_of: "length (list_of x n) = n"
+  unfolding list_of_def length_list_of' by auto
+
+lemma set_list_of': "0 < n \<Longrightarrow> set (list_of' x n xs) = insert x (set xs)"
+  apply (induction n arbitrary: x xs)
+   apply blast
+  subgoal for n x xs
+    by fastforce
+  done
+
+lemma set_list_of: 
+  "0 < n \<Longrightarrow> set (list_of x n) = {x}"
+  "set (list_of x 0) = {}"
+  unfolding list_of_def set_list_of' by auto
+
+
+(* needs a different name *)
+(* Turns a list into a list of functions, by applying a function with two arguments to each member. 
+  Then applies the list of functions sequentially beginning at some starting element and creates 
+  another list this way. This sounds like an imperative program, because it is used to simulate 
+  the execution of an imperative program (a PDDL plan). It could be implemented as a monad.*)
+fun fold_map::"('a \<Rightarrow> 'b \<Rightarrow> 'b) \<Rightarrow> 'a list \<Rightarrow> 'b \<Rightarrow> 'b list" where
+"fold_map f [] y = []" |
+"fold_map f (Cons x xs) y = Cons (f x y) (fold_map f xs (f x y))"
+
+definition fold_map'::"('a \<Rightarrow> 'b \<Rightarrow> 'b) \<Rightarrow> 'a list \<Rightarrow> 'b \<Rightarrow> 'b list" where
+"fold_map' f xs y \<equiv> 
+  let 
+    fs = map f xs
+  in foldl (\<lambda>ys f. case ys of Cons y ys \<Rightarrow> Cons (f y) (Cons y ys)) [y] fs
+"
+
+lemma tl_rev_foldl:
+  assumes "ys = Cons y' ys'"
+  shows "tl (rev (foldl (\<lambda>ys f. case ys of y # ys \<Rightarrow> f y # y # ys) (ys @ [y]) (map f xs))) 
+  = rev (foldl (\<lambda>ys f. case ys of y # ys \<Rightarrow> f y # y # ys) ys (map f xs))"
+  using assms
+proof (induction xs arbitrary: ys y' ys')
+  case Nil
+  then show ?case by simp
+next
+  case (Cons a xs)
+  have "rev (foldl (\<lambda>ys f. case ys of y # ys \<Rightarrow> f y # y # ys) ys (map f (a # xs))) = rev (foldl (\<lambda>ys f. case ys of y # ys \<Rightarrow> f y # y # ys) (f a y' # ys) (map f xs))"
+    apply (subst list.map)
+    apply (subst foldl.simps)
+    apply (subst Cons(2))
+    apply (subst list.case)
+    apply (subst Cons(2))
+    ..
+  with Cons.IH[of \<open>f a y' # ys\<close>]
+  have " tl (rev (foldl (\<lambda>ys f. case ys of y # ys \<Rightarrow> f y # y # ys) ((f a y' # ys) @ [y]) (map f xs))) = rev (foldl (\<lambda>ys f. case ys of y # ys \<Rightarrow> f y # y # ys) (f a y' # ys) (map f xs))"
+    by blast
+  thus "tl (rev (foldl (\<lambda>ys f. case ys of y # ys \<Rightarrow> f y # y # ys) (ys @ [y]) (map f (a # xs)))) 
+  = rev (foldl (\<lambda>ys f. case ys of y # ys \<Rightarrow> f y # y # ys) ys (map f (a # xs)))" 
+    apply (subst list.map)
+    apply (subst list.map)
+    apply (subst foldl.simps)
+    apply (subst foldl.simps)
+    unfolding Cons(2)
+    by auto
+qed
+
+lemma hd_rev_foldl: 
+  assumes "ys = Cons y' ys'"
+  shows "hd (rev (foldl (\<lambda>ys f. case ys of y # ys \<Rightarrow> f y # y # ys) ys (map f xs))) = hd (rev ys)"
+  using assms
+proof (induction xs arbitrary: ys y' ys')
+  case Nil
+  then show ?case by simp
+
+next
+  case (Cons a xs)
+  have 1: "hd (rev (foldl (\<lambda>ys f. case ys of y # ys \<Rightarrow> f y # y # ys) (f a y' # ys) (map f xs))) = hd (rev (f a y' # ys))"
+    using Cons.IH by blast
+  have 2: "hd (rev (foldl (\<lambda>ys f. case ys of y # ys \<Rightarrow> f y # y # ys) (f a y' # ys) (map f xs))) = hd (rev ys)" 
+    apply (subst 1)
+    apply (subst hd_rev)+
+    using Cons(2) 
+    by auto
+  show ?case 
+    apply (subst list.map)
+    apply (subst foldl.simps)
+    apply (subst Cons(2))
+    apply (subst list.case)
+    using 2 Cons(2) by simp
+qed
+
+lemma foldl_not_Nil: 
+  assumes "ys = Cons y' ys'"
+  shows "foldl (\<lambda>ys f. case ys of y # ys \<Rightarrow> f y # y # ys) ys (map f xs) \<noteq> []"
+  using assms
+  apply (induction xs arbitrary: ys y' ys')
+  by auto
+
+
+lemma fold_map_spec: "tl (rev (fold_map' f xs y)) = fold_map f xs y"
+  unfolding fold_map'_def Let_def
+proof (induction xs arbitrary: y)
+  case Nil
+  then show ?case by simp
+next
+  case (Cons a xs)
+  have "fold_map f xs (f a y) = tl (rev (foldl (\<lambda>ys f. case ys of y # ys \<Rightarrow> f y # y # ys) [f a y] (map f xs)))"
+    apply (subst Cons.IH[symmetric]) ..
+  also 
+  have "... = tl (tl (rev (foldl (\<lambda>ys f. case ys of y # ys \<Rightarrow> f y # y # ys) [f a y, y] (map f xs))))"
+    apply (subst tl_rev_foldl[where ys = "[f a y]", simplified, symmetric])
+    by auto
+  finally
+  have 1: "fold_map f xs (f a y) = tl (tl (rev (foldl (\<lambda>ys f. case ys of y # ys \<Rightarrow> f y # y # ys) [f a y, y] (map f xs))))" .
+  have 2: "tl (rev (foldl (\<lambda>ys f. case ys of y # ys \<Rightarrow> f y # y # ys) [f a y, y] (map f xs))) = rev (foldl (\<lambda>ys f. case ys of y # ys \<Rightarrow> f y # y # ys) [f a y] (map f xs))"
+    using tl_rev_foldl[where ys = "[f a y]"] by auto
+  have 3: "f a y = hd (rev (foldl (\<lambda>ys f. case ys of y # ys \<Rightarrow> f y # y # ys) [f a y] (map f xs)))" 
+    using hd_rev_foldl[of "[f a y]", symmetric] by auto
+  
+  have 4: "rev (foldl (\<lambda>ys f. case ys of y # ys \<Rightarrow> f y # y # ys) [f a y] (map f xs)) \<noteq> []" using foldl_not_Nil by fast
+  
+  have 5: "f a y # tl (rev (foldl (\<lambda>ys f. case ys of y # ys \<Rightarrow> f y # y # ys) [f a y] (map f xs))) = rev (foldl (\<lambda>ys f. case ys of y # ys \<Rightarrow> f y # y # ys) [f a y] (map f xs))"
+    apply (subst 3)
+    apply (rule hd_Cons_tl)
+    by (rule 4)
+  show ?case
+    apply (subst list.map)
+    apply (subst foldl.simps)
+    apply (subst list.case)
+    apply (subst fold_map.simps)
+    apply (subst 1)
+    apply (subst 2)+
+    using 5 by simp
+qed
+
+type_synonym 's state_sequence = "'s list"
+
+fun extend_sequence::"('comm \<Rightarrow> 's \<Rightarrow> 's) \<Rightarrow> 'comm list \<Rightarrow> 's state_sequence \<Rightarrow> 's state_sequence" where
+"extend_sequence f cs [] = []" |
+"extend_sequence f cs [s] = s # fold_map f cs s" |
+"extend_sequence f cs (s#S) = s # extend_sequence f cs S"
+
+lemma extend_sequence_fold_map: "z # fold_map f (xs @ ys) z = extend_sequence f ys (z # fold_map f xs z)"
+proof (induction xs arbitrary: ys z)
+  case Nil
+  then show ?case by simp
+next
+  case (Cons x xs)
+  have IH': "f x z # fold_map f (xs @ ys) (f x z) = extend_sequence f ys (f x z # fold_map f xs (f x z))" using Cons.IH .
+  show ?case 
+    apply -
+    apply (subst append_Cons)
+    apply (subst fold_map.simps)
+    apply (subst IH')
+    apply (subst fold_map.simps)
+    apply (subst extend_sequence.simps)
+    by simp
+qed
+
+    
+
+lemma extend_sequence_append: "extend_sequence f (xs @ ys) zs = extend_sequence f ys (extend_sequence f xs zs)"
+proof (induction zs arbitrary: xs ys)
+  case Nil
+  then show ?case by auto
+next
+  case (Cons z zs)
+  then show ?case 
+  proof (cases zs)
+    case Nil
+    show ?thesis unfolding Nil
+      apply (subst (2) extend_sequence.simps)
+      apply (subst extend_sequence_fold_map[symmetric])
+      apply (subst extend_sequence.simps)
+      by simp
+  next
+    fix z' zs'
+    assume zs: "zs = z' # zs'"
+    show ?thesis 
+      unfolding zs
+      apply (subst extend_sequence.simps)
+      apply (subst Cons.IH[simplified zs])
+      apply (subst extend_sequence.simps)
+      apply (cases zs')
+      by simp+
+  qed
+qed
+
+(* Things above this line are probably not used *)
+
+fun seq_apply::"('a \<Rightarrow> 'a) list \<Rightarrow> 'a \<Rightarrow> 'a list" where
+"seq_apply [] x = []" |
+"seq_apply (f#fs) x = f x # (seq_apply fs (f x))"
+
+find_theorems name: "foldl*fold"
+
+lemma fold_map_is_seq_apply: "fold_map f ys xs = seq_apply (map f ys) xs"
+  apply (induction ys arbitrary: xs)
+   apply simp
+  subgoal for y ys
+    apply (subst fold_map.simps)
+    apply (subst list.map)
+    apply (subst seq_apply.simps)
+    by blast
+  done
+
+fun ext_seq::"'a list \<Rightarrow> ('a \<Rightarrow> 'a) list \<Rightarrow> 'a list" where
+"ext_seq xs [] = xs" |
+"ext_seq [] fs = []" |
+"ext_seq [x] fs = x # seq_apply fs x" |
+"ext_seq (x#xs) fs = x # ext_seq xs fs"
+
+
+fun ext_seq'::"'s list \<Rightarrow> ('s \<Rightarrow> 's list) \<Rightarrow> 's list" where
+"ext_seq' [] f = []" |
+"ext_seq' [s] f = s # f s" |
+"ext_seq' (s#S) f = s # (ext_seq' S f)"
+
+fun ext_seq''::"'s list \<Rightarrow> ('s \<Rightarrow> 's list) list \<Rightarrow> 's list" where
+"ext_seq'' s [] = s" |
+"ext_seq'' s (f#fs) = ext_seq'' (ext_seq' s f) fs"
+
+lemma ext_seq'_seq_apply_is_ext_seq: "ext_seq' xs (seq_apply fs) = ext_seq xs fs"
+  apply (induction xs)
+   apply (induction fs)
+    apply simp
+   apply simp
+  subgoal for x xs
+    apply (induction xs)
+     apply (induction fs)
+      apply simp
+     apply simp
+    subgoal for x' xs'
+      apply (induction fs)
+       apply simp
+      subgoal for f fs
+        by simp
+      done
+    done
+  done
+
+(* 
+lemma ext_seq'_assoc: "ext_seq' (ext_seq' xs f) g = ext_seq' xs (\<lambda>x. ext_seq' (f x) g)"
+  apply (induction xs)
+   apply simp
+  subgoal for x xs
+    apply (induction xs)
+    apply (subst ext_seq'.simps)+ *)
+
+(* Not a monad. Extending an empty sequence behaves weirdly *)
 
 (* 
 value "KMP_search (array_of_list ''be'') (array_of_list ''ababcababdababe'')"
